Veritas.Verifier.Merkle.fsti
@@ -1,9 +1,11 @@
 module Veritas.Verifier.Merkle
 
+open FStar.Seq
 open Veritas.BinTree
 open Veritas.Hash
 open Veritas.Key
 open Veritas.Record
+open Veritas.Verifier
 open Veritas.Verifier.CorrectDefs
 open Veritas.Verifier.TSLog
 
@@ -48,6 +50,24 @@ val lemma_proving_ancestor_initial (#p:pos) (itsl: eac_ts_log p) (k:key{k <> Roo
                   not (is_desc k (mv_pointed_key (eac_merkle_value itsl (proving_ancestor itsl k))
                                                  (desc_dir k (proving_ancestor itsl k))))))
 
+(* if the proving ancestor of k is not Root, then Root points to some proper ancestor of 
+ * k along that direction *)
+val lemma_non_proving_ancestor_root (#p:pos) (itsl: eac_ts_log p) (k:key{k <> Root}):
+  Lemma (requires (Root <> proving_ancestor itsl k))
+        (ensures (is_proper_desc k Root /\
+                  mv_points_to_some (eac_merkle_value itsl Root)
+                                    (desc_dir k Root) /\
+                  is_proper_desc k (mv_pointed_key (eac_merkle_value itsl Root)
+                                                   (desc_dir k Root))))
+
+(* version of the previous lemma for non-root keys *)
+val lemma_non_proving_ancestor (#p:pos) (itsl: eac_ts_log p) (k:key{k <> Root}) (k':key{is_proper_desc k k'}):
+  Lemma (requires (k' <> proving_ancestor itsl k) /\ not (is_eac_state_init itsl k))
+        (ensures (mv_points_to_some (eac_merkle_value itsl k')
+                                    (desc_dir k k')) /\
+                 (is_proper_desc k (mv_pointed_key (eac_merkle_value itsl k')
+                                                   (desc_dir k k'))))
+
 (* when evicted as merkle the proving ancestor contains our hash *)
 val lemma_proving_ancestor_has_hash (#p:pos) (itsl: eac_ts_log p) (k:key{k<> Root}):
   Lemma (requires (is_eac_state_evicted_merkle itsl k))
@@ -62,3 +82,10 @@ val lemma_proving_ancestor_blum_bit (#p:pos) (itsl: eac_ts_log p) (k:key{k <> Ro
                                      (desc_dir k (proving_ancestor itsl k)) = 
                   is_eac_state_evicted_blum itsl k))
       
+val lemma_addm_ancestor_is_proving (#p:pos) (itsl: eac_ts_log p {length itsl > 0}):
+  Lemma (requires (AddM? (its_vlog_entry itsl (length itsl - 1))))
+        (ensures (Root <> vlog_entry_key (its_vlog_entry itsl (length itsl - 1)) /\        
+                  AddM?.k' (its_vlog_entry itsl (length itsl - 1)) = 
+                  proving_ancestor (its_prefix itsl (length itsl - 1))
+                                   (vlog_entry_key (its_vlog_entry itsl (length itsl - 1)))))
+  
